Major refactoring of borrow model

nola/iris/borrow.v
@@ -14,8 +14,8 @@ Implicit Type (FML : oFunctor) (α : lft) (q : Qp).
 (** ** Ghost state *)
 
 (** ID for a borrower/deposit/lender *)
-Local Definition bor_id := positive.
-Local Definition depo_id := positive.
+Local Definition depo_id := nat.
+Local Definition bor_id := nat.
 Local Definition lend_id := positive.
 Implicit Type (i : depo_id) (j : bor_id) (k : lend_id).
 
@@ -30,32 +30,26 @@ Local Canonical bor_modeO := leibnizO bor_mode.
 
 (** State of a borrower *)
 Local Definition bor_stOF FML : oFunctor := FML * bor_modeO.
+
 (** State of the borrowers *)
-Local Definition bor_stmOF FML := (gmapOF bor_id (bor_stOF FML)).
-
+Local Definition bor_stl FML Σ := list (bor_stOF FML $oi Σ).
 (** State of the lenders *)
-Local Definition lendmOF FML := (gmapOF lend_id FML).
-
-(** Kind of a deposit *)
-Local Definition depo_kind : Set := nat (* depth *) *' lft.
-Implicit Type e : depo_kind.
-#[warning="-redundant-canonical-projection"]
-Local Canonical depo_kindO := leibnizO depo_kind.
-
+Local Definition lend_stm FML Σ := gmap lend_id (FML $oi Σ).
 (** State of a deposit *)
-Local Definition depo_stOF FML : oFunctor :=
-  depo_kindO * bor_stmOF FML * lendmOF FML.
+Local Definition depo_st FML Σ : Type :=
+  lft *' bor_stl FML Σ *' lend_stm FML Σ.
 (** State of the deposits *)
-Local Definition depo_stmOF FML := (gmapOF depo_id (depo_stOF FML)).
+Local Notation depo_stl FML Σ := (list (depo_st FML Σ)).
 
 (** Algebra for a borrower *)
 Local Definition borRF FML := exclRF (bor_stOF FML).
 (** Algebra for a lender *)
 Local Definition lendRF FML := exclRF FML.
 (** Algebra for a deposit *)
+#[warning="-redundant-canonical-projection"]
+Local Canonical lftO := leibnizO lft.
 Local Definition depoRF FML : rFunctor :=
-  agreeRF depo_kindO *
-  gmapRF bor_id (borRF FML) * gmapRF lend_id (lendRF FML).
+  agreeRF lftO * gmapRF bor_id (borRF FML) * gmapRF lend_id (lendRF FML).
 
 (** Algebra for the borrowing machinery *)
 Local Definition borrowRF_def FML := authRF (gmapURF depo_id (depoRF FML)).
@@ -93,22 +87,22 @@ Proof. solve_inG. Qed.
 Section borrow.
   Context `{!borrowGS FML Σ}.
   Implicit Type (Px Qx : FML $oi Σ) (Pxl Qxl : list (FML $oi Σ))
-    (D : depo_stOF FML $oi Σ) (Dm : depo_stmOF FML $oi Σ)
-    (B : bor_stOF FML $oi Σ) (Bm : bor_stmOF FML $oi Σ)
-    (Pm : lendmOF FML $oi Σ).
+    (D : depo_st FML Σ) (Dl : depo_stl FML Σ)
+    (B : bor_stOF FML $oi Σ) (Bl : bor_stl FML Σ)
+    (Lm : lend_stm FML Σ).
 
   (** General borrower token *)
-  Local Definition bor_itok i j d α B : iProp Σ :=
-    own borrow_name (◯ {[i := (to_agree (d, α)', {[j := Excl B]}, ε)]}).
+  Local Definition bor_jtok i j α B : iProp Σ :=
+    own borrow_name (◯ {[i := (to_agree α, {[j := Excl B]}, ε)]}).
 
   (** Borrower token
 
     It may be a dead lifetime token, a closed borrower, or a retrieving
     reborrower *)
   Local Definition bor_tok_def α Px : iProp Σ :=
-    [†α] ∨ ∃ α' i j d, α ⊑□ α' ∗
-      (bor_itok i j d α' (Px, Clsd) ∨
-      ∃ β, [†β] ∗ bor_itok i j d α' (Px, Rebor β)).
+    [†α] ∨ ∃ α' i j, α ⊑□ α' ∗
+      (bor_jtok i j α' (Px, Clsd) ∨
+      ∃ β, [†β] ∗ bor_jtok i j α' (Px, Rebor β)).
   Local Lemma bor_tok_aux : seal bor_tok_def. Proof. by eexists. Qed.
   Definition bor_tok := bor_tok_aux.(unseal).
   Local Lemma bor_tok_unseal : bor_tok = bor_tok_def.
@@ -117,47 +111,47 @@ Section borrow.
   (** Open borrower token
 
     It keeps a live lifetime token [(r/2).[α']] at hand *)
-  Local Definition obor_dtok d α' α q Px : iProp Σ :=
-    ∃ i j r, α ⊑□ α' ∗ (r.[α'] -∗ q.[α]) ∗ (r/2).[α'] ∗
-      bor_itok i j d α' (Px, Open (r/2)).
+  Local Definition obor_itok i α' α q Px : iProp Σ :=
+    ∃ j r, α ⊑□ α' ∗ (r.[α'] -∗ q.[α]) ∗ (r/2).[α'] ∗
+      bor_jtok i j α' (Px, Open (r/2)).
   Local Definition obor_tok_def α q Px : iProp Σ :=
-    ∃ d α', obor_dtok d α' α q Px.
+    ∃ i α', obor_itok i α' α q Px.
   Local Lemma obor_tok_aux : seal obor_tok_def. Proof. by eexists. Qed.
   Definition obor_tok := obor_tok_aux.(unseal).
   Local Lemma obor_tok_unseal : obor_tok = obor_tok_def.
   Proof. exact: seal_eq. Qed.
 
   (** Lender token *)
-  Local Definition lend_itok i k d α Px : iProp Σ :=
-    own borrow_name (◯ {[i := (to_agree (d, α)', ε, {[k := Excl Px]})]}).
-  Local Definition lend_dtok d α Px : iProp Σ :=
-    ∃ i k, lend_itok i k d α Px.
+  Local Definition lend_ktok i k α Px : iProp Σ :=
+    own borrow_name (◯ {[i := (to_agree α, ε, {[k := Excl Px]})]}).
+  Local Definition lend_itok i α Px : iProp Σ :=
+    ∃ k, lend_ktok i k α Px.
   Local Definition lend_tok_def α Px : iProp Σ :=
-    ∃ α', α' ⊑□ α ∗ ∃ d, lend_dtok d α' Px.
+    ∃ α', α' ⊑□ α ∗ ∃ i, lend_itok i α' Px.
   Local Lemma lend_tok_aux : seal lend_tok_def. Proof. by eexists. Qed.
   Definition lend_tok := lend_tok_aux.(unseal).
   Local Lemma lend_tok_unseal : lend_tok = lend_tok_def.
   Proof. exact: seal_eq. Qed.
 
   (** Borrower and lender tokens are non-expansive *)
-  Local Instance bor_itok_ne {i j d α} : NonExpansive (bor_itok i j d α).
+  Local Instance bor_itok_ne {i j α} : NonExpansive (bor_jtok i j α).
   Proof.
-    unfold bor_itok=> ????. do 2 f_equiv. apply singleton_ne.
+    unfold bor_jtok=> ????. do 2 f_equiv. apply singleton_ne.
     do 2 apply pair_ne=>//. apply singleton_ne. by f_equiv.
   Qed.
   #[export] Instance bor_tok_ne {α} : NonExpansive (bor_tok α).
   Proof. rewrite bor_tok_unseal. solve_proper. Qed.
-  #[export] Instance obor_dtok_ne {d α' α q} :
-    NonExpansive (obor_dtok d α' α q).
+  #[export] Instance obor_itok_ne {i α' α q} :
+    NonExpansive (obor_itok i α' α q).
   Proof. solve_proper. Qed.
   #[export] Instance obor_tok_ne {α q} : NonExpansive (obor_tok α q).
   Proof. rewrite obor_tok_unseal. solve_proper. Qed.
-  Local Instance lend_itok_ne {i k d α} : NonExpansive (lend_itok i k d α).
+  Local Instance lend_ktok_ne {i k α} : NonExpansive (lend_ktok i k α).
   Proof.
-    unfold lend_itok=> ????. do 2 f_equiv. apply singleton_ne.
+    unfold lend_ktok=> ????. do 2 f_equiv. apply singleton_ne.
     apply pair_ne=>//. apply singleton_ne. by f_equiv.
   Qed.
-  Local Instance lend_dtok_ne {d α} : NonExpansive (lend_dtok d α).
+  Local Instance lend_itok_ne {i α} : NonExpansive (lend_itok i α).
   Proof. solve_proper. Qed.
   #[export] Instance lend_tok_ne {α} : NonExpansive (lend_tok α).
   Proof. rewrite lend_tok_unseal. solve_proper. Qed.
@@ -182,14 +176,14 @@ Section borrow.
   Proof.
     rewrite bor_tok_unseal. iIntros "#? [?|b]".
     { iLeft. by iApply lft_sincl_dead. }
-    iDestruct "b" as (????) "[#? b]". iRight. iExists _, _, _, _. iFrame "b".
+    iDestruct "b" as (???) "[#? b]". iRight. iExists _, _, _. iFrame "b".
     by iApply lft_sincl_trans.
   Qed.
   Lemma obor_tok_lft {α β q r Px} :
     β ⊑□ α -∗ (q.[α] -∗ r.[β]) -∗ obor_tok α q Px -∗ obor_tok β r Px.
   Proof.
     rewrite obor_tok_unseal. iIntros "#? →β".
-    iDestruct 1 as (? α' ???) "[#?[→α o]]". iExists _, _, _, _, _. iFrame "o".
+    iDestruct 1 as (? α' ??) "[#?[→α o]]". iExists _, _, _, _. iFrame "o".
     iSplit; [by iApply lft_sincl_trans|]. iIntros "α'". iApply "→β".
     by iApply "→α".
   Qed.
@@ -199,182 +193,224 @@ Section borrow.
     by iApply lft_sincl_trans.
   Qed.
 
-  (** Token for [depo_stm] *)
-  Local Definition depo_st_R D : depoRF FML $ri Σ :=
-    let '(e, Bm, Pm) := D in (to_agree e, Excl <$> Bm, Excl <$> Pm).
-  Arguments depo_st_R _ /.
-  Local Definition depo_stm_tok Dm : iProp Σ :=
-    own borrow_name (● (depo_st_R <$> Dm : gmapR _ _)).
-
   (** Lemma for [to_bor_itoks] *)
-  Local Lemma bor_insert_op {i j e B Bm} :
+  Local Lemma bor_insert_op {i j α B Bm} :
     Bm !! j = None →
-    (◯ {[i := (to_agree e, Excl <$> <[j:=B]> Bm, ε)]} : borrowRF_def _ $ri _) ≡
-      ◯ {[i := (to_agree e, {[j:=Excl B]}, ε)]} ⋅
-      ◯ {[i := (to_agree e, Excl <$> Bm, ε)]}.
+    (◯ {[i := (to_agree α, Excl <$> <[j:=B]> Bm, ε)]} : borrowRF_def _ $ri _) ≡
+      ◯ {[i := (to_agree α, {[j:=Excl B]}, ε)]} ⋅
+      ◯ {[i := (to_agree α, Excl <$> Bm, ε)]}.
   Proof.
     move=> eq. rewrite fmap_insert -auth_frag_op. f_equiv. rewrite singleton_op.
     apply: singletonM_proper.
     split; [split|]=>/=; [by rewrite agree_idemp| |done].
     rewrite insert_singleton_op; [done|]. by rewrite lookup_fmap eq.
   Qed.
-  (** Get [bor_itok]s out of [own] *)
-  Local Lemma to_bor_itoks {i d α Bm} :
-    own borrow_name (◯ {[i := (to_agree (d, α)', Excl <$> Bm, ε)]}) ⊢
-      [∗ map] j ↦ B ∈ Bm, bor_itok i j d α B.
+  (** Get [bor_jtok]s out of [own] *)
+  Local Lemma to_bor_jtoks {i α Bm} :
+    own borrow_name (◯ {[i := (to_agree α, Excl <$> Bm, ε)]}) ⊢
+      [∗ map] j ↦ B ∈ Bm, bor_jtok i j α B.
   Proof.
-    induction (Bm : gmap _ _) as [|j B Bm' ? IH] using map_ind.
+    induction Bm as [|j B Bl' ? IH] using map_ind.
     { rewrite big_sepM_empty. by iIntros. }
     rewrite big_sepM_insert; [|done]. rewrite -IH bor_insert_op; [|done].
     iIntros "[$$]".
   Qed.
 
-  (** Lemma for [to_lend_itoks] *)
-  Local Lemma lend_insert_op {i k e Px Pm} :
-    Pm !! k = None →
-    (◯ {[i := (to_agree e, ε, Excl <$> <[k:=Px]> Pm)]} : borrowRF_def _ $ri _) ≡
-      ◯ {[i := (to_agree e, ε, {[k:=Excl Px]})]} ⋅
-      ◯ {[i := (to_agree e, ε, Excl <$> Pm)]}.
+  (** Lemma for [to_lend_ktoks] *)
+  Local Lemma lend_insert_op {i k α Px Lm} :
+    Lm !! k = None →
+    (◯ {[i := (to_agree α, ε, Excl <$> <[k:=Px]> Lm)]} : borrowRF_def _ $ri _) ≡
+      ◯ {[i := (to_agree α, ε, {[k:=Excl Px]})]} ⋅
+      ◯ {[i := (to_agree α, ε, Excl <$> Lm)]}.
     move=> eq. rewrite fmap_insert -auth_frag_op. f_equiv. rewrite singleton_op.
     apply: singletonM_proper.
     split; [split|]=>/=; [by rewrite agree_idemp|done|].
     rewrite insert_singleton_op; [done|]. by rewrite lookup_fmap eq.
   Qed.
-  (** Get [lend_itok]s out of [own] *)
-  Local Lemma to_lend_itoks {i d α Pm} :
-    own borrow_name (◯ {[i := (to_agree (d, α)', ε, Excl <$> Pm)]}) ⊢
-      [∗ map] k ↦ Px ∈ Pm, lend_itok i k d α Px.
+  (** Get [lend_ktok]s out of [own] *)
+  Local Lemma to_lend_ktoks {i α Lm} :
+    own borrow_name (◯ {[i := (to_agree α, ε, Excl <$> Lm)]}) ⊢
+      [∗ map] k ↦ Px ∈ Lm, lend_ktok i k α Px.
   Proof.
-    induction (Pm : gmap _ _) as [|k Px Pm' ? IH] using map_ind.
+    induction (Lm : gmap _ _) as [|k Px Lm' ? IH] using map_ind.
     { rewrite big_sepM_empty. by iIntros. }
     rewrite big_sepM_insert; [|done]. rewrite -IH lend_insert_op; [|done].
     iIntros "[$$]".
   Qed.
 
-  (** Create [bor_itok]s and [lend_itok]s w.r.t. [depo_stm_tok] *)
-  Local Lemma depo_stm_bor_lend_new {Dm} d α Pxl Qxl :
-    depo_stm_tok Dm -∗ |==> ∃ i,
-      let Bm := map_by _ (fmap (M:=list) (λ Px, (Px, Clsd)) Pxl) in
-      let Qm := map_by _ Qxl in
-      depo_stm_tok (<[i := ((d, α)', Bm, Qm)]> Dm) ∗
-      ([∗ map] j ↦ B ∈ Bm, bor_itok i j d α B) ∗
-      [∗ map] k ↦ Qx ∈ Qm, lend_itok i k d α Qx.
+  (** [depo_st] to [depoRF] *)
+  Local Definition of_depo_st (D : depo_st FML Σ) : depoRF FML $ri Σ :=
+    let '(α, Bl, Lm)' := D in
+    (to_agree α, Excl <$> list_to_gmap Bl, Excl <$> Lm).
+  (** Auxiliary definition for performance *)
+  Local Definition depoR FML Σ : cmra :=
+    prodR (prodR (agreeR lftO)
+      (gmapR bor_id (exclR (prodO (FML $oi Σ) bor_modeO))))
+      (gmapR lend_id (exclR (FML $oi Σ))).
+  Local Definition of_depo_st' : depo_st FML Σ → depoR FML Σ := of_depo_st.
+  Local Lemma eq_of_depo_st' : of_depo_st = of_depo_st'. Proof. done. Qed.
+
+  (** [depo_stk] to [gmap] over [depoRF] *)
+  Local Definition of_depo_stl (Dl : depo_stl FML Σ)
+    : gmapR depo_id (depoRF FML $ri Σ) := list_to_gmap (of_depo_st <$> Dl).
+  (** Token for [depo_stl] *)
+  Local Definition depo_stl_tok Dl : iProp Σ :=
+    own borrow_name (● of_depo_stl Dl).
+
+  (** [!!] over [of_depo_stl] *)
+  Local Lemma lookup_of_depo_stl {Dl i} :
+    of_depo_stl Dl !! i = of_depo_st <$> (Dl !! i).
+  Proof. by rewrite lookup_list_to_gmap list_lookup_fmap. Qed.
+  (** [of_depo_stl] over [insert] *)
+  Local Lemma of_depo_stl_insert {Dl i D} : i < length Dl →
+    of_depo_stl (<[i := D]> Dl) = <[i := of_depo_st D]> (of_depo_stl Dl).
   Proof.
-    iIntros "●". iExists (fresh (dom Dm)).
+    move=> ?. rewrite /of_depo_stl list_fmap_insert.
+    rewrite list_to_gmap_insert; by [|rewrite length_fmap].
+  Qed.
+
+  (** Create [bor_jtok]s and [lend_itok]s w.r.t. [depo_stl_tok] *)
+  Local Lemma depo_stl_bor_lend_new {Dl α} Pxl Qxl :
+    let i := length Dl in let Bl := (λ Px, (Px, Clsd)) <$> Pxl in
+    depo_stl_tok Dl -∗ |==>
+      depo_stl_tok (Dl ++ [(α, Bl, map_by _ Qxl)']) ∗
+      ([∗ list] B ∈ Bl, ∃ j, bor_jtok i j α B) ∗
+      [∗ list] Qx ∈ Qxl, lend_itok i α Qx.
+  Proof.
+    move=> ? Bl. iIntros "●".
     iMod (own_update with "●") as "[$[b l]]"; last first.
-    { iModIntro. iDestruct (to_bor_itoks (d:=d) with "b") as "$".
-      iApply (to_lend_itoks with "l"). }
-    rewrite -auth_frag_op singleton_op fmap_insert.
-    have <- : ∀ x y, ((to_agree (d, α)', x, y) : depoRF _ $ri _) ≡
-      ((to_agree (d, α)', x, ε) : depoRF _ $ri _) ⋅ (to_agree (d, α)', ε, y).
+    { iModIntro. iSplitL "b".
+      - erewrite to_bor_jtoks, (big_sepM_list_to_gmap Bl). iStopProof.
+        do 3 f_equiv. iIntros "$".
+      - iStopProof. erewrite to_lend_ktoks. apply big_sepM_map_by'. }
+    rewrite -auth_frag_op singleton_op.
+    have <- : ∀ x y, ((to_agree α, x, y) : depoRF _ $ri _) ≡
+      ((to_agree α, x, ε) : depoRF _ $ri _) ⋅ (to_agree α, ε, y).
     { split; [split|]=>/=; by
         [rewrite agree_idemp|rewrite left_id|rewrite right_id]. }
+    rewrite /of_depo_stl fmap_snoc list_to_gmap_snoc length_fmap.
     apply auth_update_alloc, alloc_singleton_local_update.
-    - rewrite lookup_fmap. apply fmap_None, not_elem_of_dom_1, is_fresh.
+    - by rewrite lookup_of_depo_stl fmap_None lookup_ge_None.
     - split; [split|]=>/=; [done|by apply: gmap_fmap_valid..].
   Qed.
 
-  (** Lemmas for [depo_stm_lend_agree] and [depo_stm_bor_agree] *)
-  Local Lemma depo_stm_own_agree' {Dm i d α Bx Pxx n} :
-    ✓{n} (● (depo_st_R <$> Dm) ⋅ ◯ {[i := (to_agree (d, α)', Bx, Pxx)]}
+  (** Lemmas for [depo_stl_lend_agree] and [depo_stl_bor_agree] *)
+  Local Lemma depo_stl_own_agree {Dl i α Bxm Pxm n} :
+    ✓{n} (● of_depo_stl Dl ⋅ ◯ {[i := (to_agree α, Bxm, Pxm)]}
       : borrowRF_def _ $ri _) →
-    ∃ Bm Pm, (Dm !! i = Some ((d, α)', Bm, Pm)) ∧
-      Bx ≼{n} Excl <$> Bm ∧ Pxx ≼{n} Excl <$> Pm.
+    ∃ Bl Lm, Dl !! i = Some (α, Bl, Lm)' ∧
+      Bxm ≼{n} Excl <$> list_to_gmap Bl ∧ Pxm ≼{n} Excl <$> Lm.
   Proof.
     move=> /auth_both_validN/proj1/singleton_includedN_l.
     move=> [?[/Some_equiv_eq[?[++]] /Some_includedN_total +]].
-    move=> /lookup_fmap_Some[[[dα Bm]Pm] [<- ?]] <-.
+    rewrite lookup_of_depo_stl=> /fmap_Some[[?[??]][? ->]]<-.
     move=> /prod_includedN[/prod_includedN/=[+ ?] ?].
-    move=> /to_agree_includedN/leibniz_equiv_iff ?. subst. by exists Bm, Pm.
-  Qed.
-  Local Lemma depo_stm_own_agree {Dm i d α Bx Pxx} :
-    depo_stm_tok Dm -∗
-    own borrow_name (◯ {[i := (to_agree (d, α)', Bx, Pxx)]}) -∗
-    ∃ Bm Pm, ⌜Dm !! i = Some ((d, α)', Bm, Pm)⌝ ∧
-      Bx ≼ Excl <$> Bm ∧ Pxx ≼ Excl <$> Pm.
-  Proof.
-    iIntros "● o". iDestruct (own_valid_2 with "● o") as "?". iStopProof.
-    unfold internal_included. uPred.unseal.
-    by split=> ?? _ /depo_stm_own_agree'.
+    move=> /to_agree_includedN/leibniz_equiv_iff ?. subst. by eexists _, _.
   Qed.
 
-  (** Agreement between [depo_stm_tok] and [lend_itok] *)
-  Local Lemma depo_stm_lend_agree {Dm i k d α Px} :
-    depo_stm_tok Dm -∗ lend_itok i k d α Px -∗ ∃ Bm Pm Px',
-      ⌜Dm !! i = Some ((d, α)', Bm, Pm)⌝ ∧ ⌜Pm !! k = Some Px'⌝ ∧ Px' ≡ Px.
+  (** Agreement between [depo_stl_tok] and [lend_itok] *)
+  Local Lemma depo_stl_lend_agree' {Dl i k α Px n} :
+    ✓{n} (● of_depo_stl Dl ⋅ ◯ {[i := (to_agree α, ε, {[k := Excl Px]})]}
+      : borrowRF_def _ $ri _) → ∃ Bl Lm Px',
+      Dl !! i = Some (α, Bl, Lm)' ∧ Lm !! k = Some Px' ∧ Px' ≡{n}≡ Px.
   Proof.
-    iIntros "● l".
-    iDestruct (depo_stm_own_agree with "● l") as (Bm Pm ?) "[_?]".
-    iStopProof. unfold internal_included. uPred.unseal. split=> n ? _.
-    repeat unfold uPred_holds=>/=.
-    move /singleton_includedN_l=>
-      [?[/Some_equiv_eq[?[/lookup_fmap_Some[Px'[<-?]]<-]]/Excl_includedN incl]].
-    by exists Bm, Pm, Px'.
+    move=> /depo_stl_own_agree[?[?[?[_ +]]]].
+    move=> /singleton_includedN_l
+      [?[/Some_equiv_eq[?[/lookup_fmap_Some[Px'[<-?]]<-]]/Excl_includedN ?]].
+    by eexists _, _, _.
   Qed.
-  (** Delete a lender w.r.t. [depo_stm_tok] *)
-  Local Lemma depo_stm_lend_delete {Dm i k d α Bm Pm Px} :
-    Dm !! i = Some ((d, α)', Bm, Pm) →
-    depo_stm_tok Dm -∗ lend_itok i k d α Px ==∗
-      depo_stm_tok (<[i := ((d, α)', Bm, delete k Pm)]> Dm).
+  Local Lemma depo_stl_lend_agree {Dl i k α Px} :
+    depo_stl_tok Dl -∗ lend_ktok i k α Px -∗ ∃ Bl Lm Px',
+      ⌜Dl !! i = Some (α, Bl, Lm)'⌝ ∧ ⌜Lm !! k = Some Px'⌝ ∧ Px' ≡ Px.
   Proof.
-    move=> ?. iIntros "● l". iMod (own_update_2 with "● l") as "[$_]"; [|done].
-    apply auth_update. rewrite fmap_insert.
+    iIntros "● l". iDestruct (own_valid_2 with "● l") as "?".
+    iStopProof. unfold internal_included. uPred.unseal.
+    by split=> ?? _ /depo_stl_lend_agree'.
+  Qed.
+
+  (** Delete a lender w.r.t. [depo_stl_tok] *)
+  Local Lemma depo_stl_lend_delete {Dl i k α Bl Lm Px} :
+    Dl !! i = Some (α, Bl, Lm)' →
+    depo_stl_tok Dl -∗ lend_ktok i k α Px ==∗
+      depo_stl_tok (<[i := (α, Bl, delete k Lm)']> Dl).
+  Proof.
+    move=> eq. iIntros "● l". iMod (own_update_2 with "● l") as "[$_]"; [|done].
+    apply auth_update. rewrite of_depo_stl_insert; [|by apply: lookup_lt_Some].
     eapply (singleton_local_update _ _ _ _ _ (_,_,_)).
-    { rewrite lookup_fmap_Some. by eexists _. }
+    { by rewrite lookup_of_depo_stl eq. }
     apply prod_local_update; [apply prod_local_update|]=>/=; [done..|].
     rewrite fmap_delete. apply: delete_local_update; last first.
     { by rewrite lookup_singleton. } exact _.
   Qed.
-  (** Add lenders w.r.t. [depo_stm_tok] *)
-  Local Lemma depo_stm_lend_add {Dm i d α Bm Pm} Qxl :
-    Dm !! i = Some ((d, α)', Bm, Pm) →
-    depo_stm_tok Dm ==∗
-      depo_stm_tok (<[i := ((d, α)', Bm, map_with Pm Qxl)]> Dm) ∗
-      [∗ map] k ↦ Qx ∈ map_without Pm Qxl, lend_itok i k d α Qx.
+
+  (** Add lenders w.r.t. [depo_stl_tok] *)
+  Local Lemma depo_stl_lend_add' {α Bl Lm Qxl} :
+    (Some (of_depo_st' (α, Bl, Lm)'), None) ~l~>
+    (Some (of_depo_st' (α, Bl, map_with Lm Qxl)'),
+      Some (to_agree α, ε, Excl <$> map_without Lm Qxl)).
   Proof.
-    move=> eq. iIntros "●". iMod (own_update with "●") as "[$ ?]"; last first.
-    { iModIntro. by iApply to_lend_itoks. }
-    rewrite fmap_insert. apply auth_update_alloc, gmap_local_update.
-    move=> i'. case: (decide (i = i'))=> [<-|?]; last first.
-    { rewrite lookup_insert_ne; [|done]. by rewrite lookup_singleton_ne. }
-    rewrite lookup_empty lookup_fmap eq !lookup_insert /=.
-    apply local_update_unital=> n ?[/=??]. rewrite left_id=> <-. split.
+    apply local_update_unital=> n ?[/=??]. rewrite (left_id None)=> <-. split.
     { split; [done|]. by apply: gmap_fmap_valid. }
     rewrite -Some_op. f_equiv.
     split; [split|]=>/=; [by rewrite agree_idemp|by rewrite left_id|].
     rewrite gmap_op_disj; [|by apply map_disjoint_fmap, map_without_disj].
     by rewrite -map_fmap_union -map_with_without.
   Qed.
-
-  (** Agreement between [depo_stm_tok] and [bor_itok] *)
-  Local Lemma depo_stm_bor_agree {Dm i j d α B} :
-    depo_stm_tok Dm -∗ bor_itok i j d α B -∗ ∃ Bm Pm B',
-      ⌜Dm !! i = Some ((d, α)', Bm, Pm)⌝ ∧ ⌜Bm !! j = Some B'⌝ ∧ B' ≡ B.
+  Local Lemma depo_stl_lend_add {Dl i α Bl Lm} Qxl :
+    Dl !! i = Some (α, Bl, Lm)' →
+    depo_stl_tok Dl ==∗
+      depo_stl_tok (<[i := (α, Bl, map_with Lm Qxl)']> Dl) ∗
+      [∗ map] k ↦ Qx ∈ map_without Lm Qxl, lend_ktok i k α Qx.
   Proof.
-    iIntros "● B".
-    iDestruct (depo_stm_own_agree with "● B") as (Bm Pm ?) "[? _]".
-    iStopProof. unfold internal_included. uPred.unseal. split=> n ? _.
-    repeat unfold uPred_holds=>/=.
-    move /singleton_includedN_l=>
-      [?[/Some_equiv_eq[?[/lookup_fmap_Some[B'[<-?]]<-]]/Excl_includedN incl]].
-    by exists Bm, Pm, B'.
+    move=> eq. iIntros "●". iMod (own_update with "●") as "[$ ?]"; last first.
+    { iModIntro. by iApply to_lend_ktoks. }
+    rewrite of_depo_stl_insert; [|by apply: lookup_lt_Some].
+    apply auth_update_alloc, gmap_local_update. move=> i'.
+    case: (decide (i = i'))=> [<-|?]; last first.
+    { rewrite lookup_insert_ne; [|done]. by rewrite lookup_singleton_ne. }
+    rewrite lookup_empty lookup_of_depo_stl eq !lookup_insert.
+    apply depo_stl_lend_add'.
   Qed.
-  (** Update the borrower state w.r.t. [depo_stm_tok] *)
-  Local Lemma depo_stm_bor_stupd {Dm i j d α Bm Pm B B'} :
-    Dm !! i = Some ((d, α)', Bm, Pm) →
-    depo_stm_tok Dm -∗ bor_itok i j d α B ==∗
-      depo_stm_tok (<[i := ((d, α)', <[j := B']> Bm, Pm)]> Dm) ∗
-      bor_itok i j d α B'.
+
+  (** Agreement between [depo_stl_tok] and [bor_jtok] *)
+  Local Lemma depo_stl_bor_agree' {Dl i j α B n} :
+    ✓{n} (● of_depo_stl Dl ⋅ ◯ {[i := (to_agree α, {[j := Excl B]}, ε)]}
+      : borrowRF_def _ $ri _) → ∃ Bl Lm B',
+      Dl !! i = Some (α, Bl, Lm)' ∧ Bl !! j = Some B' ∧ B' ≡{n}≡ B.
+  Proof.
+    move=> /depo_stl_own_agree[?[?[?[+ _]]]].
+    move=> /singleton_includedN_l[?
+      [/Some_equiv_eq[?[/lookup_fmap_Some[B'[<- +]]<-]]/Excl_includedN incl]].
+    rewrite lookup_list_to_gmap=> ?. by eexists _, _, _.
+  Qed.
+  Local Lemma depo_stl_bor_agree {Dl i j α B} :
+    depo_stl_tok Dl -∗ bor_jtok i j α B -∗ ∃ Bl Lm B',
+      ⌜Dl !! i = Some (α, Bl, Lm)'⌝ ∧ ⌜Bl !! j = Some B'⌝ ∧ B' ≡ B.
+  Proof.
+    iIntros "● B". iDestruct (own_valid_2 with "● B") as "?". iStopProof.
+    unfold internal_included. uPred.unseal.
+    by split=> n ? _ /depo_stl_bor_agree'.
+  Qed.
+
+  (** Update the borrower state w.r.t. [depo_stl_tok] *)
+  Local Lemma depo_stl_bor_stupd {Dl i j α Bl Lm B B'} :
+    Dl !! i = Some (α, Bl, Lm)' →
+    depo_stl_tok Dl -∗ bor_jtok i j α B ==∗
+      depo_stl_tok (<[i := (α, <[j := B']> Bl, Lm)']> Dl) ∗
+      bor_jtok i j α B'.
   Proof.
     move=> eq. iIntros "● B".
-    iDestruct (depo_stm_bor_agree with "● B") as (??? eq' eq'') "#_".
-    move: eq' eq''. rewrite eq. move=> [<- _] ?.
+    iDestruct (depo_stl_bor_agree with "● B") as (??? eq' eq'') "#_".
+    move: eq' eq''. rewrite eq. move=> [<-_] ?.
     iMod (own_update_2 with "● B") as "[$$]"; [|done].
-    apply auth_update. rewrite fmap_insert. eapply singleton_local_update.
-    { rewrite lookup_fmap_Some. by eexists _. }
+    apply auth_update. rewrite of_depo_stl_insert; [|by apply: lookup_lt_Some].
+    eapply singleton_local_update. { by rewrite lookup_of_depo_stl eq. }
     apply prod_local_update; [apply prod_local_update|]=>/=; [done| |done].
+    rewrite list_to_gmap_insert; [|by apply: lookup_lt_Some].
     rewrite fmap_insert. apply: singleton_local_update.
-    { rewrite lookup_fmap_Some. by eexists _. } by apply exclusive_local_update.
+    { rewrite lookup_fmap_Some. eexists _.
+      split; by [|rewrite lookup_list_to_gmap]. }
+    by apply exclusive_local_update.
   Qed.
 End borrow.
 
@@ -383,31 +419,31 @@ End borrow.
 Section borrow.
   Context `{!borrowGS FML Σ}.
   Implicit Type (M : iProp Σ → iProp Σ) (sm : FML $oi Σ -d> iProp Σ)
-    (Px Qx : FML $oi Σ) (D : depo_stOF FML $oi Σ) (Dm : depo_stmOF FML $oi Σ)
-    (B : bor_stOF FML $oi Σ) (Bm : bor_stmOF FML $oi Σ)
-    (Pm : lendmOF FML $oi Σ).
+    (Px Qx : FML $oi Σ) (D : depo_st FML Σ) (Dl : depo_stl FML Σ)
+    (B : bor_stOF FML $oi Σ) (Bl : bor_stl FML Σ) (Lm : lend_stm FML Σ).
 
   (** World satisfaction for a borrower *)
-  Local Definition bor_wsat sm d α B : iProp Σ :=
+  Local Definition bor_wsat sm i α B : iProp Σ :=
     let '(Qx, b) := B in match b with
     | Clsd => sm Qx | Open q => q.[α]
-    | Rebor β => ⌜β ⊑ α⌝ ∗ ∃ d', ⌜d < d'⌝ ∗ lend_dtok d' β Qx
+    | Rebor β => ⌜β ⊑ α⌝ ∗ ∃ i', ⌜i < i'⌝ ∗ lend_itok i' β Qx
     end.
 
-  (** World satisfaction for a deposit *)
-  Local Definition depo_wsat_in M sm d α Bm Pm : iProp Σ :=
-    ([∗ map] B ∈ Bm, bor_wsat sm d α B) ∗
-    ([†α] -∗ ([∗ map] '(Qx, _) ∈ Bm, sm Qx) -∗ M ([∗ map] Px ∈ Pm, sm Px)%I).
-  Local Definition depo_wsat_dead M sm α Pm : iProp Σ :=
-    [†α] ∗ M ([∗ map] Px ∈ Pm, sm Px)%I.
-  Local Definition depo_wsat M sm d α Bm Pm : iProp Σ :=
-    depo_wsat_in M sm d α Bm Pm ∨ depo_wsat_dead M sm α Pm.
+  (** World satisfaction for a deposit, borrowed or retrieved *)
+  Local Definition depo_wsat_bor M sm i α Bl Lm : iProp Σ :=
+    ([∗ list] B ∈ Bl, bor_wsat sm i α B) ∗
+    ([†α] -∗ ([∗ list] '(Qx, _) ∈ Bl, sm Qx) -∗ M ([∗ map] Px ∈ Lm, sm Px)%I).
+  Local Definition depo_wsat_ret M sm α Lm : iProp Σ :=
+    [†α] ∗ M ([∗ map] Px ∈ Lm, sm Px)%I.
+  Local Definition depo_wsat M sm i α Bl Lm : iProp Σ :=
+    depo_wsat_bor M sm i α Bl Lm ∨ depo_wsat_ret M sm α Lm.
 
   (** World satisfaction for the borrowing machinery *)
-  Local Definition borrow_wsat' M sm Dm :=
-    ([∗ map] '((d, α)', Bm, Pm) ∈ Dm, depo_wsat M sm d α Bm Pm)%I.
+  Local Definition borrow_lwsat M sm Dl : iProp Σ :=
+    depo_stl_tok Dl ∗
+    [∗ list] i ↦ '(α, Bl, Lm)' ∈ Dl, depo_wsat M sm i α Bl Lm.
   Local Definition borrow_wsat_def M sm : iProp Σ :=
-    ∃ Dm, depo_stm_tok Dm ∗ borrow_wsat' M sm Dm.
+    ∃ Dl, borrow_lwsat M sm Dl.
   Local Definition borrow_wsat_aux : seal borrow_wsat_def.
   Proof. by eexists. Qed.
   Definition borrow_wsat := borrow_wsat_aux.(unseal).
@@ -423,13 +459,13 @@ Section borrow.
       (=) ==> (≡{n}≡)) depo_wsat.
   Proof.
     move=> ?? eqv ?????<-??<-??<-??<-.
-    unfold depo_wsat, depo_wsat_in, depo_wsat_dead.
+    unfold depo_wsat, depo_wsat_bor, depo_wsat_ret.
     (repeat f_equiv); [done|..]; apply eqv; solve_proper.
   Qed.
   #[export] Instance borrow_wsat_ne {n} :
     Proper (((≡{n}≡) ==> (≡{n}≡)) ==> (≡{n}≡) ==> (≡{n}≡)) borrow_wsat.
   Proof.
-    rewrite borrow_wsat_unseal /borrow_wsat_def /borrow_wsat'=> ??????.
+    rewrite borrow_wsat_unseal /borrow_wsat_def /borrow_lwsat. move=> ??????.
     repeat f_equiv. by apply depo_wsat_ne.
   Qed.
 
@@ -437,33 +473,34 @@ Section borrow.
   Local Instance depo_wsat_mono :
     Mono (OT:=_ → _ : bi) (OT':=_ → _ → _ → _ → _ → _ : bi) depo_wsat.
   Proof.
-    move=> ?? to ?????. unfold depo_wsat, depo_wsat_in, depo_wsat_dead.
+    move=> ?? to ?????. unfold depo_wsat, depo_wsat_bor, depo_wsat_ret.
     repeat f_equiv; exact: to.
   Qed.
   #[export] Instance borrow_wsat_mono :
     Mono (OT:=_ → _ : bi) (OT':=_ → _ : bi) borrow_wsat.
   Proof.
-    rewrite borrow_wsat_unseal /borrow_wsat_def /borrow_wsat'=> ????.
+    rewrite borrow_wsat_unseal /borrow_wsat_def /borrow_lwsat. move=> ????.
     repeat f_equiv. by apply: depo_wsat_mono.
   Qed.
 
   Context `{!GenUpd M, !GenUpdB M, !NonExpansive sm}.
 
-  (** Create new borrowers and lenders with a specific depth *)
-  Local Lemma bor_lend_tok_new_list' d α Pxl Qxl :
+  (** Create new borrowers and lenders *)
+  Local Lemma bor_lend_tok_new_list' {Dl} α Pxl Qxl :
     ([∗ list] Px ∈ Pxl, sm Px) -∗
-    ([†α] -∗ ([∗ list] Px ∈ Pxl, sm Px) -∗ M ([∗ list] Qx ∈ Qxl, sm Qx)%I)
-      =[borrow_wsat M sm]=∗
-      ([∗ list] Px ∈ Pxl, bor_tok α Px) ∗ [∗ list] Qx ∈ Qxl, lend_dtok d α Qx.
+    ([†α] -∗ ([∗ list] Px ∈ Pxl, sm Px) -∗ M ([∗ list] Qx ∈ Qxl, sm Qx)%I) -∗
+    borrow_lwsat M sm Dl ==∗ ∃ D,
+      borrow_lwsat M sm (Dl ++ [D]) ∗ ([∗ list] Px ∈ Pxl, bor_tok α Px) ∗
+      [∗ list] Qx ∈ Qxl, lend_itok (length Dl) α Qx.
   Proof.
-    rewrite borrow_wsat_unseal bor_tok_unseal. iIntros "Pxl →Qxl [%Dm[● Dm]]".
-    iMod (depo_stm_bor_lend_new d α Pxl Qxl with "●") as (?) "[●[b l]]".
-    iModIntro. rewrite !big_sepM_map_by' big_sepL_fmap.
-    iSplitR "b l"; last first; [iSplitL "b"; iStopProof; do 3 f_equiv;
-      iIntros "[% ?]"; [|by iExists _, _]|].
-    { iRight. iExists _, _, _, _. iSplitR; by [iApply lft_sincl_refl|iLeft]. }
-    iExists _. iFrame "●". iApply (big_sepM_insert_2 with "[Pxl →Qxl] Dm").
-    iLeft. iSplitL "Pxl"; by rewrite !big_sepM_map_by big_sepL_fmap.
+    rewrite bor_tok_unseal. iIntros "Pxl →Qxl [● Dl]".
+    iMod (depo_stl_bor_lend_new Pxl Qxl with "●") as "($ & b & $)".
+    iModIntro. iSplitR "b"; last first.
+    { iStopProof. rewrite big_sepL_fmap. do 3 f_equiv.
+      iIntros "[% b]". iRight. iExists _, _, _.
+      iSplitR; by [iApply lft_sincl_refl|iLeft]. }
+    rewrite big_sepL_snoc /=. iFrame "Dl". iLeft.
+    iSplitL "Pxl"; [|rewrite ?big_sepM_map_by]; by rewrite big_sepL_fmap.
   Qed.
 
   (** Create new borrowers and lenders *)
@@ -473,8 +510,8 @@ Section borrow.
       =[borrow_wsat M sm]=∗
       ([∗ list] Px ∈ Pxl, bor_tok α Px) ∗ [∗ list] Qx ∈ Qxl, lend_tok α Qx.
   Proof.
-    iIntros "Pxl →Qxl".
-    iMod (bor_lend_tok_new_list' 0 with "Pxl →Qxl") as "[$ ?]".
+    rewrite borrow_wsat_unseal. iIntros "Pxl →Qxl [% W]".
+    iMod (bor_lend_tok_new_list' with "Pxl →Qxl W") as (?) "($ & $ & ?)".
     iModIntro. iStopProof. do 3 f_equiv. iIntros "l". rewrite lend_tok_unseal.
     iExists _. iSplit; [by iApply lft_sincl_refl|]. by iExists _.
   Qed.
@@ -492,247 +529,173 @@ Section borrow.
       =[borrow_wsat M sm]=∗ [∗ list] Qx ∈ Qxl, lend_tok α Qx.
   Proof.
     rewrite lend_tok_unseal borrow_wsat_unseal.
-    iIntros "[%α'[#?[%d[%i[%k l]]]]] PQ [%Dm[● Dm]]".
-    iDestruct (depo_stm_lend_agree with "● l") as (Bm Pm Px' ? ?) "#eqv".
+    iIntros "(%α' & #? & %i & %k & l) PQ [%Dl[● Dl]]".
+    iDestruct (depo_stl_lend_agree with "● l") as (??? eq ?) "#eqv".
     iRewrite -"eqv" in "PQ".
-    iMod (depo_stm_lend_delete with "● l") as "●"; [done|].
-    iMod (depo_stm_lend_add Qxl with "●") as "[● ls]".
-    { apply (lookup_insert (M:=gmap _)). }
+    iMod (depo_stl_lend_delete with "● l") as "●"; [done|].
+    iMod (depo_stl_lend_add Qxl with "●") as "[● ls]".
+    { apply list_lookup_insert. by apply: lookup_lt_Some. }
     iModIntro. iSplitR "ls"; last first.
     { rewrite big_sepM_map_without'. iApply (big_sepL_impl with "ls").
-      iIntros "!> %% ⊑ [% ?]". iExists _. iSplit; [done|]. by iExists _, _, _. }
-    iExists _. iFrame "●". rewrite insert_insert.
-    iDestruct (big_sepM_insert_acc with "Dm") as "[D →Dm]"; [done|]=>/=.
-    iApply "→Dm". iDestruct "D" as "[[Bm →Pm]|[† Pm]]".
-    - iLeft. iFrame "Bm". iIntros "† Bm". iMod ("→Pm" with "† Bm") as "Pm".
-      rewrite big_sepM_map_with.
-      iDestruct (big_sepM_delete with "Pm") as "[? $]"; [done|]. by iApply "PQ".
-    - iRight. iFrame "†". iMod "Pm". rewrite big_sepM_map_with.
-      iDestruct (big_sepM_delete with "Pm") as "[Px $]"; [done|].
-      by iApply "PQ".
+      iIntros "!> %% ⊑ [% ?]". iExists _. iSplit; [done|]. by iExists _, _. }
+    iExists _. iFrame "●". rewrite list_insert_insert.
+    iDestruct (big_sepL_insert_acc with "Dl") as "[D →Dl]"; [done|]=>/=.
+    iApply "→Dl". clear eq. iDestruct "D" as "[[Bl →Lm]|[† Lm]]".
+    - iLeft. iFrame "Bl". iIntros "† Bl".
+      iMod ("→Lm" with "† Bl") as "Lm". rewrite big_sepM_map_with.
+      iDestruct (big_sepM_delete with "Lm") as "[? $]"; by [|iApply "PQ"].
+    - iRight. iFrame "†". iMod "Lm". rewrite big_sepM_map_with.
+      iDestruct (big_sepM_delete with "Lm") as "[Px $]"; by [|iApply "PQ"].
   Qed.
 
   (** [depo_wsat] with deposits under [α] retrieved *)
-  Local Definition depo_wsat_ret M sm d' α β Bm Pm : iProp Σ :=
-    if decide (β ⊑ α) then depo_wsat_dead M sm β Pm
-    else depo_wsat M sm d' β Bm Pm.
+  Local Definition depo_wsat_ret' M sm α i β Bl Lm : iProp Σ :=
+    if decide (β ⊑ α)
+      then depo_wsat_ret M sm β Lm else depo_wsat M sm i β Bl Lm.
+  (** [borrow_wsat_ret] with deposits after [Dl], retrieved under [α] *)
+  Local Definition borrow_wsat_ret M sm α Dl : iProp Σ :=
+    ∃ Dl', depo_stl_tok (Dl ++ Dl') ∗
+      [∗ list] i ↦ '(β, Bl, Lm)' ∈ Dl',
+        depo_wsat_ret' M sm α (length Dl + i) β Bl Lm.
 
-  (** Filter [depo_stm] with a depth *)
-  Local Notation dep_of D := D.1.1.1'.
-  Local Notation filter_ge d := (filter (λ iD, d ≤ dep_of iD.2)).
-  Local Notation filter_lt d := (filter (λ iD, dep_of iD.2 < d)).
-  Local Notation filter_eq d := (filter (λ iD, dep_of iD.2 = d)).
-  (** [borrow_wsat] with deposits under [d] and [α] retrieved *)
-  Local Definition borrow_wsat_dret M sm Dm d α : iProp Σ :=
-    ∃ Dm', ⌜filter_lt d Dm' = filter_lt d Dm⌝ ∗ depo_stm_tok Dm' ∗
-      [∗ map] '((d', β)', Bm, Pm) ∈ filter_ge d Dm',
-        depo_wsat_ret M sm d' α β Bm Pm.
-  (** [borrow_wsat] with deposits under [α] retrieved *)
-  Local Definition borrow_wsat_ret M sm Dm := borrow_wsat_dret M sm Dm 0.
-
-  (** Retrieve from [borrow_wsat_dret] using [lend_dtok] *)
-  Local Lemma lend_dtok_dret_retrieve {Dm d d' α β Px} : d ≤ d' → β ⊑ α →
-    lend_dtok d' β Px -∗ modw M (borrow_wsat_dret M sm Dm d α) (sm Px).
+  (** Retrieve using [lend_itok] under [borrow_wsat_ret] *)
+  Local Lemma lend_itok_ret_retrieve {i Dl α β Px} : length Dl ≤ i → β ⊑ α →
+    lend_itok i β Px -∗ modw M (borrow_wsat_ret M sm α Dl) (sm Px).
   Proof.
-    move=> ??. iIntros "[%[% l]] [%Dm'[%[● Dm']]]".
-    iDestruct (depo_stm_lend_agree with "● l") as (Bm Pm Px' eq ?) "#eqv".
-    iRewrite -"eqv". iDestruct (big_sepM_insert_acc with "Dm'") as "[D →Dm']".
-    { rewrite map_lookup_filter_Some. split; [done|]=>/=. lia. }
-    rewrite /depo_wsat_ret decide_True; [|done]. iDestruct "D" as "[† >Pm]".
-    iDestruct (big_sepM_delete with "Pm") as "[$ Pm]"; [done|]=>/=.
-    iMod (depo_stm_lend_delete with "● l") as "●"; [done..|]. iModIntro.
-    iExists _. iFrame "●". iSplit.
-    { iPureIntro. rewrite map_filter_insert_False /=; [|lia].
-      rewrite map_filter_delete_not; [done|]. rewrite eq. move=> ?[<-]/=. lia. }
-    rewrite map_filter_insert_True /=; [|done]. iApply "→Dm'".
-    rewrite decide_True; [|done]. by iFrame.
+    move=> ??. iIntros "[% l] [%Dl'[● Dl']]".
+    iDestruct (depo_stl_lend_agree with "● l") as (??? eq ?) "#eqv".
+    iRewrite -"eqv". move: (eq). rewrite lookup_app_r; [|done]=> ?.
+    iDestruct (big_sepL_insert_acc with "Dl'") as "[D →Dl']"; [done|]=>/=.
+    iMod (depo_stl_lend_delete with "● l") as "●"; [done|].
+    rewrite insert_app_r_alt; [|done]. iFrame "●".
+    rewrite /depo_wsat_ret' decide_True; [|done].
+    iDestruct "D" as "[† >Lm]". iModIntro.
+    iDestruct (big_sepM_delete with "Lm") as "[$ Lm]"; [done|]=>/=.
+    iApply "→Dl'". rewrite decide_True; [|done]. by iFrame.
   Qed.
-  Local Lemma lend_dtok_ret_retrieve {Dm d α Px} :
-    lend_dtok d α Px -∗ modw M (borrow_wsat_ret M sm Dm α) (sm Px).
-  Proof. apply lend_dtok_dret_retrieve; [lia|done]. Qed.
 
-  (** Retrieve from [bor_wsat] *)
-  Local Lemma bor_wsat_retrieve {Dm d α β Px b} : β ⊑ α →
-    [†β] -∗ bor_wsat sm d β (Px, b) -∗
-      modw M (borrow_wsat_dret M sm Dm (S d) α) (sm Px).
+  (** Retrieve from [bor_wsat] under [borrow_wsat_ret] *)
+  Local Lemma bor_wsat_retrieve {Dl D α β Px b} : β ⊑ α →
+    [†β] -∗ bor_wsat sm (length Dl) β (Px, b) -∗
+      modw M (borrow_wsat_ret M sm α (Dl ++ [D])) (sm Px).
   Proof.
-    move=> ?. iIntros "† B". case b=> [|q|?]/=; [done|..].
+    move=> ?. iIntros "† B". case b=> [|q|?]/=. { done. }
     { iDestruct (lft_live_dead with "B †") as %[]. }
     iDestruct "B" as (???) "l".
-    iApply (lend_dtok_dret_retrieve with "l"); [lia|]. by etrans.
+    iApply (lend_itok_ret_retrieve with "l"); [|by etrans].
+    rewrite length_app /=. lia.
   Qed.
   (** Retrieve from [bor_wsat]s *)
-  Local Lemma bor_wsats_retrieve {Dm d α β Bl} : β ⊑ α →
-    [†β] -∗ ([∗ list] B ∈ Bl, bor_wsat sm d β B) -∗
-      modw M (borrow_wsat_dret M sm Dm (S d) α)
+  Local Lemma bor_wsatl_retrieve {Dl D α β Bl} : β ⊑ α →
+    [†β] -∗ ([∗ list] B ∈ Bl, bor_wsat sm (length Dl) β B) -∗
+      modw M (borrow_wsat_ret M sm α (Dl ++ [D]))
         ([∗ list] '(Px, _) ∈ Bl, sm Px)%I.
   Proof.
-    move=> ?. elim: Bl; [by iIntros|]. move=>/= [??]Bl IH. iIntros "#† [B Bl]".
+    move=> ?. elim: Bl; [by iIntros|]. move=>/= [??] Bl IH. iIntros "#† [B Bl]".
     iMod (IH with "† Bl") as "$". by iApply bor_wsat_retrieve.
   Qed.
 
-  (** Retrieve from [depo_wsat] *)
-  Local Lemma depo_wsat_retrieve {Dm d α β Bm Pm} : β ⊑ α →
-    [†β] -∗ depo_wsat M sm d β Bm Pm -∗
-      modw M (borrow_wsat_dret M sm Dm (S d) α) (depo_wsat_dead M sm β Pm)%I.
+  (** Retrieve from [depo_wsat] and enrich [borrow_wsat_ret] *)
+  Local Lemma depo_wsat_retrieve' {Dl α β Bl Lm} :
+    [†α] -∗ depo_wsat M sm (length Dl) β Bl Lm -∗
+      modw M (borrow_wsat_ret M sm α (Dl ++ [(β, Bl, Lm)']))
+        (depo_wsat_ret' M sm α (length Dl) β Bl Lm).
   Proof.
-    move=> ?. iIntros "#† [[Bl →Pm]|?]"; [|done]. iFrame "†". iApply modw_fold.
-    iDestruct ("→Pm" with "†") as "→Pm".
-    setoid_rewrite (big_sepM_map_to_list_snd Bm).
-    iMod (bor_wsats_retrieve with "† Bl") as "Bl"; [done..|].
-    iDestruct ("→Pm" with "Bl") as "$". by iIntros.
+    unfold depo_wsat_ret'. case (decide (β ⊑ α)); [|by iIntros "_ _ ?"]=> ?.
+    iIntros "#† [[Bl →Lm]|?]"; [|done]. rewrite lft_incl_dead; [|done].
+    iFrame "†". iApply modw_fold. iDestruct ("→Lm" with "†") as "→Lm".
+    iMod (bor_wsatl_retrieve with "† Bl") as "Bl"; [done|].
+    iMod ("→Lm" with "Bl") as "$". by iIntros "$".
   Qed.
+  Local Lemma depo_wsat_retrieve {Dl α β Bl Lm} :
+    [†α] -∗ depo_wsat M sm (length Dl) β Bl Lm -∗
+    borrow_wsat_ret M sm α (Dl ++ [(β, Bl, Lm)']) -∗
+      M (borrow_wsat_ret M sm α Dl).
+  Proof.
+    iIntros "† W D".
+    iMod (depo_wsat_retrieve' with "† W D") as "[(% & ● & Dl') D]". iModIntro.
+    setoid_rewrite length_app. setoid_rewrite <-Nat.add_assoc.
+    rewrite -app_assoc /=. iFrame "● Dl'". by rewrite (right_id 0).
+  Qed.
+
   (** Retrieve from [depo_wsat]s *)
-  Local Lemma depo_wsats_retrieve {Dm d α Dl} :
-    [†α] -∗ ([∗ list] D ∈ Dl,
-      if decide (dep_of D = d) then let '((d', β)', Bm, Pm) := D in
-        depo_wsat M sm d' β Bm Pm else True) -∗
-      modw M (borrow_wsat_dret M sm Dm (S d) α)
-        ([∗ list] D ∈ Dl,
-          if decide (dep_of D = d) then let '((d', β)', Bm, Pm) := D in
-            depo_wsat_ret M sm d' α β Bm Pm else True)%I.
+  Local Lemma depo_wsatl_retrieve {α Dl} : [†α] -∗
+    ([∗ list] i ↦ '(β, Bl, Lm)' ∈ Dl, depo_wsat M sm i β Bl Lm) -∗
+    borrow_wsat_ret M sm α Dl -∗
+    M (borrow_wsat_ret M sm α []).
   Proof.
-    elim: Dl; [by iIntros|]. move=> [[[d' β]?]?] Dl IH /=. iIntros "#† [D Dl]".
-    iMod (IH with "† Dl") as "$". iApply modw_fold. rewrite /depo_wsat_ret.
-    case: (decide (β ⊑ α)); [|done]=> ?. rewrite lft_incl_dead; [|done].
-    case: (decide (d' = d)); [|done]=> ->. by iApply depo_wsat_retrieve.
-  Qed.
-
-  (** Lemmas for [borrow_wsat_eq_retrieve] *)
-  Local Lemma filter_eq_lt d Dm :
-    filter_eq d Dm = filter_eq d (filter_lt (S d) Dm).
-  Proof.
-    rewrite map_filter_filter.
-    apply (map_filter_ext (M:=gmap _))=> ?[[??]?]/=?. lia.
-  Qed.
-  Local Lemma filter_lt_lt d Dm :
-    filter_lt d Dm = filter_lt d (filter_lt (S d) Dm).
-  Proof.
-    rewrite map_filter_filter.
-    apply (map_filter_ext (M:=gmap _))=> ?[[??]?]/=?. lia.
-  Qed.
-  (** Retrieve from [borrow_wsat'] over [filter_eq] *)
-  Local Lemma borrow_wsat'_eq_retrieve {Dm d α} :
-    [†α] -∗ borrow_wsat' M sm (filter_eq d Dm) -∗
-      borrow_wsat_dret M sm Dm (S d) α -∗
-      M (borrow_wsat_dret M sm Dm d α).
-  Proof.
-    iIntros "† eq ret".
-    rewrite /borrow_wsat' big_sepM_filter' /= big_sepM_map_to_list_snd.
-    iMod (depo_wsats_retrieve with "† eq ret") as "[ret eq]".
-    iModIntro. iDestruct "ret" as (Dm' eq) "[● ret]". iExists _. iFrame "●".
-    rewrite -big_sepM_map_to_list_snd -big_sepM_filter''.
-    rewrite filter_eq_lt (filter_lt_lt d Dm) -!eq -filter_eq_lt -filter_lt_lt.
-    iSplit; [done|].
-    iApply (big_sepM_filter_complement (λ iD, dep_of iD.2 ≠ d)). iStopProof.
-    do 2 f_equiv; rewrite map_filter_filter;
-      apply (map_filter_ext (M:=gmap _))=>/=; lia.
-  Qed.
-  (** Lemma for [borrow_wsat_lt_retrieve] *)
-  Local Lemma borrow_wsat'_lt_S_split d Dm :
-    borrow_wsat' M sm (filter_lt (S d) Dm) ⊣⊢
-      borrow_wsat' M sm (filter_eq d Dm) ∗ borrow_wsat' M sm (filter_lt d Dm).
-  Proof.
-    rewrite /borrow_wsat' (big_sepM_filter_complement (λ iD, dep_of iD.2 = d)).
-    do 2 f_equiv; rewrite map_filter_filter;
-      apply (map_filter_ext (M:=gmap _))=>/=; lia.
-  Qed.
-  (** Retrieve from [borrow_wsat'] over [filter_lt] *)
-  Local Lemma borrow_wsat'_lt_retrieve {Dm d α} :
-    [†α] -∗ borrow_wsat' M sm (filter_lt d Dm) -∗
-      borrow_wsat_dret M sm Dm d α -∗ M (borrow_wsat_ret M sm Dm α).
-  Proof.
-    elim: d; [by iIntros|]=> ? IH. rewrite borrow_wsat'_lt_S_split.
-    iIntros "#† [eq lt] ret".
-    iMod (borrow_wsat'_eq_retrieve with "† eq ret") as "ret".
-    iApply (IH with "† lt ret").
-  Qed.
-
-  (** Find large enough [d] that empties [filter_ge d Dm] *)
-  Local Lemma filter_ge_empty Dm : ∃ d, filter_ge d Dm = ∅.
-  Proof.
-    induction (Dm : gmap _ _) as [|i[[[d' ?] ?]?]?? [d eq]] using map_ind;
-      [by exists 0|].
-    exists (d `max` S d'). rewrite map_filter_insert_False /=; [|lia].
-    rewrite map_filter_delete -(delete_empty i). f_equal.
-    apply (f_equal (filter_ge (S d'))) in eq. move: eq.
-    rewrite map_filter_filter map_filter_empty=> <-.
-    apply map_filter_ext=> ?[[??]?]/=. lia.
+    rewrite /= -(reverse_involutive Dl). move: (reverse Dl)=> Dl'.
+    iIntros "#†". iInduction Dl' as [|[?[??]] Dl'] "IH"; [by iIntros|]=>/=.
+    rewrite reverse_cons. rewrite big_sepL_snoc. iIntros "[Dl D] ret".
+    iMod (depo_wsat_retrieve with "† D ret") as "ret".
+    iApply ("IH" with "Dl ret").
   Qed.
   (** Retrieve from [borrow_wsat] *)
   Local Lemma borrow_wsat_retrieve {α} :
-    [†α] -∗ borrow_wsat M sm -∗ M (∃ Dm, borrow_wsat_ret M sm Dm α).
+    [†α] -∗ borrow_wsat M sm -∗ M (borrow_wsat_ret M sm α []).
   Proof.
-    rewrite borrow_wsat_unseal. iIntros "† [%Dm[● Dm]]". iExists Dm.
-    case: (filter_ge_empty Dm)=> d eq.
-    iApply (borrow_wsat'_lt_retrieve (d:=d) with "† [Dm] [●]").
-    - iDestruct (big_sepM_filter_complement with "Dm") as "[$ _]".
-    - iExists _. iFrame "●". rewrite eq. by iSplit.
-  Qed.
-  (** [borrow_wsat_ret] into [borrow_wsat] *)
-  Local Lemma borrow_wsat_from_ret {Dm α} :
-    borrow_wsat_ret M sm Dm α ⊢ borrow_wsat M sm.
-  Proof.
-    rewrite borrow_wsat_unseal. iIntros "[%[_[● ?]]]". iExists _. iFrame "●".
-    rewrite map_filter_id; [|lia]. iStopProof. unfold borrow_wsat'.
-    do 2 f_equiv. move=> [[[? β]?]?]. unfold depo_wsat_ret.
-    case: (decide (β ⊑ α))=> ?; [|done]. iIntros. by iRight.
+    rewrite borrow_wsat_unseal. iIntros "† [%Dl[● Dl]]".
+    iApply (depo_wsatl_retrieve with "† Dl"). iExists []. rewrite app_nil_r.
+    by iFrame.
   Qed.
 
-  (** Retrive using [lend_dtok] *)
-  Local Lemma lend_dtok_retrieve {d α Px} :
-    [†α] -∗ lend_dtok d α Px -∗ modw M (borrow_wsat M sm) (sm Px).
+  (** Retrive using [lend_itok] *)
+  Local Lemma lend_itok_retrieve {i α Px} :
+    [†α] -∗ lend_itok i α Px -∗ modw M (borrow_wsat M sm) (sm Px).
   Proof.
-    iIntros "† l W". iMod (borrow_wsat_retrieve with "† W") as (Dm) "ret".
-    iMod (lend_dtok_ret_retrieve with "l ret") as "[ret $]". iModIntro.
-    by iApply borrow_wsat_from_ret.
+    iIntros "† l W". rewrite {2}borrow_wsat_unseal.
+    iMod (borrow_wsat_retrieve with "† W") as "ret".
+    iMod (lend_itok_ret_retrieve with "l ret") as "[ret $]"=>/=; [lia|done|].
+    iModIntro. iDestruct "ret" as (?) "[$ ?]"=>/=. iStopProof. do 2 f_equiv.
+    move=> [β ?]. unfold depo_wsat_ret'. case (decide (β ⊑ α)); [|done].
+    iIntros. by iRight.
   Qed.
   (** Retrive using [lend_tok] *)
   Lemma lend_tok_retrieve {α Px} :
     [†α] -∗ lend_tok α Px -∗ modw M (borrow_wsat M sm) (sm Px).
   Proof.
-    rewrite lend_tok_unseal. iIntros "† [%α'[⊑[%d l]]]".
+    rewrite lend_tok_unseal. iIntros "† [%α'[⊑[%i l]]]".
     iDestruct (lft_sincl_dead with "⊑ †") as "†".
-    by iApply (lend_dtok_retrieve with "† l").
+    by iApply (lend_itok_retrieve with "† l").
   Qed.
 
   (** [depo_wsat] with a live lifetime token *)
-  Local Lemma depo_wsat_tok {d α Bm Pm q} :
-    q.[α] -∗ depo_wsat M sm d α Bm Pm -∗ q.[α] ∗ depo_wsat_in M sm d α Bm Pm.
+  Local Lemma depo_wsat_tok {i α Bl Lm q} :
+    q.[α] -∗ depo_wsat M sm i α Bl Lm -∗ q.[α] ∗ depo_wsat_bor M sm i α Bl Lm.
   Proof.
     iIntros "α [$|[† _]]"; [done|].
     iDestruct (lft_live_dead with "α †") as %[].
   Qed.
 
   (** [bor_wsat] is non-expansive over the borrower state *)
-  Local Instance bor_wsat_ne_st {d α} : NonExpansive (bor_wsat sm d α).
+  Local Instance bor_wsat_ne_st {i α} : NonExpansive (bor_wsat sm i α).
   Proof.
     move=> ?[?[|?|?]][?[|?|?]][//=eqv /leibniz_equiv_iff].
     { by rewrite eqv. } { by move=> [<-]. }
-    move=> [<-]. unfold lend_dtok, lend_itok. do 10 f_equiv.
-    apply singleton_ne. split=>/=; [done|]. by rewrite eqv.
+    move=> [<-]. do 4 f_equiv. by apply lend_itok_ne.
   Qed.
 
   (** Update the borrower state to [Open q] *)
-  Local Lemma bor_open_core {i j d α Px b q} :
-    q.[α] -∗ bor_itok i j d α (Px, b) =[borrow_wsat M sm]=∗
-      obor_tok α q Px ∗ bor_wsat sm d α (Px, b).
+  Local Lemma bor_open_core {i j α Px b q} :
+    q.[α] -∗ bor_jtok i j α (Px, b) =[borrow_wsat M sm]=∗
+      obor_tok α q Px ∗ bor_wsat sm i α (Px, b).
   Proof.
-    rewrite borrow_wsat_unseal. iIntros "[α α'] b [%Dm[● Dm]]".
-    iDestruct (depo_stm_bor_agree with "● b") as (Bm Qm [Px' b'] ??) "#eqv".
-    iDestruct (big_sepM_insert_acc with "Dm") as "[D →Dm]"; [done|].
-    iDestruct (depo_wsat_tok with "α D") as "[α [Bm →Qm]]".
-    iMod (depo_stm_bor_stupd with "● b") as "[● o]"; [done..|]. iRewrite -"eqv".
-    iDestruct (big_sepM_insert_acc with "Bm") as "[$ →Bm]"; [done|]. iModIntro.
+    rewrite borrow_wsat_unseal. iIntros "[α α'] b [%Dl[● Dl]]".
+    iDestruct (depo_stl_bor_agree with "● b") as (Bl Lm [??]? eq) "#eqv".
+    iDestruct (big_sepL_insert_acc with "Dl") as "[D →Dl]"; [done|].
+    iDestruct (depo_wsat_tok with "α D") as "[α [Bl →Qm]]".
+    iMod (depo_stl_bor_stupd with "● b") as "[● o]"; [done..|]. iRewrite -"eqv".
+    iDestruct (big_sepL_insert_acc with "Bl") as "[$ →Bl]"; [done|]. iModIntro.
     iSplitR "α o"; last first.
-    { rewrite obor_tok_unseal. iExists _, _, _, _, _.
+    { rewrite obor_tok_unseal. iExists _, _, _, _.
       iSplitR; [iApply lft_sincl_refl|]. iSplitR; [by iIntros|]. iFrame. }
-    iExists _. iFrame "●". iApply "→Dm". iLeft.
-    iSplitR "→Qm"=>/=; [by iApply "→Bm"|]. iIntros "† big".
-    iApply ("→Qm" with "†").
-    iApply (big_sepM_insert_override_1 with "big"); [done|].
-    rewrite prod_equivI /=. iDestruct "eqv" as "[eqv _]". iRewrite "eqv".
-    by iIntros.
+    iExists _. iFrame "●". iApply "→Dl". iLeft.
+    iSplitR "→Qm"=>/=; [by iApply "→Bl"|]. iIntros "† big".
+    iApply ("→Qm" with "†"). rewrite -{2}(list_insert_id _ _ _ eq).
+    iDestruct (big_sepL_insert_acc _ _ j with "big") as "[Px big]".
+    { apply list_lookup_insert. by apply: lookup_lt_Some. }
+    setoid_rewrite list_insert_insert. iApply "big". rewrite prod_equivI /=.
+    iDestruct "eqv" as "[eqv ?]". iRewrite "eqv". by iIntros.
   Qed.
   (** Open a borrower *)
   Lemma bor_tok_open {α q Px} :
@@ -741,58 +704,70 @@ Section borrow.
   Proof.
     rewrite bor_tok_unseal. iIntros "α [†|b]".
     { by iDestruct (lft_live_dead with "α †") as %[]. }
-    iDestruct "b" as (????) "[#⊑ b]".
+    iDestruct "b" as (???) "[#⊑ b]".
     iMod (lft_sincl_live_acc with "⊑ α") as (r) "[α' →α]".
     iDestruct "b" as "[b|[%β[#† r]]]".
     - iMod (bor_open_core with "α' b") as "[o $]". iApply modw_fold.
       iApply (obor_tok_lft with "⊑ →α o").
     - iMod (bor_open_core with "α' r") as "[o [%[%[_ l]]]]".
       iDestruct (obor_tok_lft with "⊑ →α o") as "$". iApply modw_fold.
-      iApply (lend_dtok_retrieve with "† l").
+      iApply (lend_itok_retrieve with "† l").
   Qed.
 
-  (** Turn [obor_dtok] to a reborrower using [lend_dtok] *)
-  Local Lemma obor_dtok_reborrow {d α' α q Px β d'} : d < d' → β ⊑ α' →
-    obor_dtok d α' α q Px -∗ lend_dtok d' β Px =[borrow_wsat M sm]=∗
+  (** Turn [obor_itok] to a reborrower using [lend_itok] *)
+  Local Lemma obor_itok_reborrow {i α' α q Px β i'} : i < i' → β ⊑ α' →
+    obor_itok i α' α q Px -∗ lend_itok i' β Px =[borrow_wsat M sm]=∗
       q.[α] ∗ ([†β] -∗ bor_tok α Px).
   Proof.
     rewrite borrow_wsat_unseal=> ??.
-    iDestruct 1 as (i j r) "(#⊑ & →α & α' & o)".
-    iIntros "[%i'[%k l]] [%Dm [● Dm]]".
-    iDestruct (depo_stm_bor_agree with "● o") as (Bm Pm B' ??) "#eqv".
-    iDestruct (big_sepM_insert_acc with "Dm") as "[D →Dm]"; [done|]=>/=.
-    iMod (depo_stm_bor_stupd (B':=(_, Rebor β)) with "● o") as "[● r]";
+    iIntros "(%j & %r & #⊑ & →α & α' & o) [%k l] [%Dl [● Dl]]".
+    iDestruct (depo_stl_bor_agree with "● o") as (Bl Lm B' ? eq) "#eqv".
+    iDestruct (big_sepL_insert_acc with "Dl") as "[D →Dl]"; [done|]=>/=.
+    iMod (depo_stl_bor_stupd (B':=(_, Rebor β)) with "● o") as "[● r]";
       [done..|]. iModIntro.
-    iDestruct (depo_wsat_tok with "α' D") as "[α'[Bm →Pm]]".
-    iDestruct (big_sepM_insert_acc with "Bm") as "[B' →Bm]"; [done|].
+    iDestruct (depo_wsat_tok with "α' D") as "[α'[Bl →Lm]]".
+    iDestruct (big_sepL_insert_acc with "Bl") as "[B' →Bl]"; [done|].
     iRewrite "eqv" in "B'"=>/=.
     iDestruct ("→α" with "[$α' $B']") as "$". iSplitR "r"; last first.
-    { iIntros "†". rewrite bor_tok_unseal. iRight. iExists _, _, _, _.
+    { iIntros "†". rewrite bor_tok_unseal. iRight. iExists _, _, _.
       iFrame "⊑". iRight. iExists _. by iSplit. }
-    iExists _. iFrame "●". iApply "→Dm". iLeft. iSplitR "→Pm".
-    { iApply "→Bm". iSplit; [done|]. iExists _. iSplit; by [|iExists _, _]. }
-    iIntros "† big". iApply ("→Pm" with "†").
-    iApply (big_sepM_insert_override_1 with "big"); [done|].
+    iExists _. iFrame "●". iApply "→Dl". iLeft. iSplitR "→Lm".
+    { iApply "→Bl". iSplit; [done|]. iExists _. iSplit; by [|iExists _]. }
+    iIntros "† big". iApply ("→Lm" with "†").
+    rewrite -{2}(list_insert_id _ _ _ eq).
+    iDestruct (big_sepL_insert_acc _ _ j with "big") as "[Px big]".
+    { apply list_lookup_insert. by apply: lookup_lt_Some. }
+    setoid_rewrite list_insert_insert. iApply "big".
     rewrite prod_equivI /=. iDestruct "eqv" as "[eqv _]". case B'=>/= ??.
-    iRewrite "eqv". by iIntros.
+    by iRewrite "eqv".
   Qed.
 
   (** Lemmas for [obor_tok_merge_subdiv] *)
-  Local Lemma obor_dtok_lft_sincl {d' α α' q Px} :
-    obor_dtok d' α α' q Px ⊢ α' ⊑□ α.
-  Proof. iDestruct 1 as (???) "[$ _]". Qed.
-  Local Lemma obor_toks_dtoks_bound {αqPxl β} :
-    ([∗ list] '(α, q, Px)' ∈ αqPxl, β ⊑□ α ∗ obor_tok α q Px) ⊢ ∃ d γ,
+  Local Lemma obor_itok_lft_sincl {i α α' q Px} :
+    obor_itok i α α' q Px ⊢ α' ⊑□ α.
+  Proof. iDestruct 1 as (??) "[$ _]". Qed.
+  Local Lemma obor_itok_lt {i α α' q Px Dl} :
+    obor_itok i α α' q Px -∗ borrow_lwsat M sm Dl -∗ ⌜i < length Dl⌝.
+  Proof.
+    iIntros "(% & % & _ & _ & _ & o) [● _]".
+    iDestruct (depo_stl_bor_agree with "● o") as (?????) "_". iPureIntro.
+    by apply: lookup_lt_Some.
+  Qed.
+  Local Lemma obor_toks_itoks_bound {αqPxl β Dl} :
+    ([∗ list] '(α, q, Px)' ∈ αqPxl, β ⊑□ α ∗ obor_tok α q Px) -∗
+    borrow_lwsat M sm Dl -∗ ∃ γ, borrow_lwsat M sm Dl ∗
       β ⊑□ γ ∗ γ ⊑□ β ∗
-      [∗ list] '(α, q, Px)' ∈ αqPxl, ∃ d' α',
-        ⌜d' < d ∧ γ ⊑ α'⌝ ∗ obor_dtok d' α' α q Px.
+      [∗ list] '(α, q, Px)' ∈ αqPxl, ∃ i α',
+        ⌜i < length Dl ∧ γ ⊑ α'⌝ ∗ obor_itok i α' α q Px.
   Proof.
     elim: αqPxl=>/=.
-    { iIntros. iExists 0, β. iSplit; [|iSplit=>//]; iApply lft_sincl_refl. }
-    move=> [α[Px q]] αqPxl ->. rewrite obor_tok_unseal.
-    iIntros "[[#βα (%d & %α' & o)] (%d' & %γ & #? & #? & big)]".
-    iDestruct (obor_dtok_lft_sincl with "o") as "#?".
-    iExists (S d `max` d'), (γ ⊓ α'). iSplit; [|iSplit].
+    { iIntros "_ $". iExists β. iSplit; [|iSplit=>//]; iApply lft_sincl_refl. }
+    rewrite obor_tok_unseal. move=> [α[Px q]] αqPxl IH.
+    iIntros "[[#βα (%i' & %α' & o)] big] W".
+    iDestruct (obor_itok_lt with "o W") as %?.
+    iDestruct (IH with "big W") as (γ) "($ & #⊑ & #⊑' & big)".
+    iDestruct (obor_itok_lft_sincl with "o") as "#?". iExists (γ ⊓ α').
+    iSplit; [|iSplit].
     { iApply lft_sincl_meet_intro; [done|].
       by iApply lft_sincl_trans; [|done]. }
     { iApply lft_sincl_trans; [iApply lft_sincl_meet_l|done]. }
@@ -800,7 +775,7 @@ Section borrow.
     { iExists _, _. iFrame "o". iPureIntro. split; [lia|].
       exact lft_incl_meet_r. }
     iClear "#". iStopProof. do 3 f_equiv.
-    iDestruct 1 as (d'' α'' [??]) "o". iExists _, _. iFrame "o". iPureIntro.
+    iDestruct 1 as (??[??]) "o". iExists _, _. iFrame "o". iPureIntro.
     split; [lia|]. etrans; [|done]. exact lft_incl_meet_l.
   Qed.
   (** Merge and subdivide/reborrow borrowers *)
@@ -813,19 +788,21 @@ Section borrow.
       ([∗ list] '(α, q, Px)' ∈ αqPxl, q.[α] ∗ ([†β] -∗ bor_tok α Px)) ∗
       [∗ list] Qx ∈ Qxl, bor_tok β Qx.
   Proof.
-    rewrite/= obor_toks_dtoks_bound.
-    iIntros "(%d & %γ & #⊑ & #⊑' & αqPxl) Qxl →Px".
-    iMod (bor_lend_tok_new_list' d γ Qxl ((λ '(_, _, Px)', Px) <$> αqPxl)
-      with "Qxl [→Px]") as "[bl ll]"=>/=.
+    rewrite borrow_wsat_unseal. iIntros "big Qxl →Px [%Dl W]".
+    iDestruct (obor_toks_itoks_bound with "big W")
+      as (?) "(W & #⊑ & #⊑' & αqPxl)".
+    iMod (bor_lend_tok_new_list' γ Qxl ((λ '(_, _, Px)', Px) <$> αqPxl)
+      with "Qxl [→Px] W") as (?) "(W & bl & ll)"=>/=.
     { iIntros "† Qxl". iDestruct (lft_sincl_dead with "⊑ †") as "†".
       rewrite big_sepL_fmap. iApply ("→Px" with "† Qxl"). }
-    iSplitR "bl"; last first.
+    rewrite assoc. iSplitR "bl"; last first.
     { iModIntro. iApply (big_sepL_impl with "bl"). iIntros "!> %% _".
       by iApply bor_tok_lft. }
-    iInduction αqPxl as [|[α[q Px]]αqPxl] "IH"=>/=; [done|].
+    iInduction αqPxl as [|[α[q Px]]αqPxl] "IH"=>/=; [by iFrame|].
     iDestruct "αqPxl" as "[big αqPxl]". iDestruct "big" as (??[??]) "o".
-    iDestruct "ll" as "[l ll]". iMod ("IH" with "αqPxl ll") as "$".
-    iMod (obor_dtok_reborrow with "o l") as "[$ →b]"; [lia|done|].
+    iDestruct "ll" as "[l ll]". iMod ("IH" with "αqPxl W ll") as "[W $]".
+    rewrite -borrow_wsat_unseal.
+    iMod (obor_itok_reborrow with "o l W") as "[$[$ →b]]"; [lia|done|].
     iModIntro. iIntros "†". iApply "→b". by iApply (lft_sincl_dead with "[] †").
   Qed.
   (** Subdivide/reborrow a borrower *)
@@ -871,8 +848,8 @@ Lemma borrow_wsat_alloc `{!borrowGpreS FML Σ} :
   ⊢ |==> ∃ _ : borrowGS FML Σ, lft_wsat ∗ ∀ M sm, borrow_wsat M sm.
 Proof.
   iMod lft_wsat_alloc as (?) "W".
-  iMod (own_alloc (● (∅ : gmap _ _) : borrowRF_def FML $ri Σ)) as (γ) "●";
+  iMod (own_alloc (● ∅ : borrowRF_def FML $ri Σ)) as (γ) "●";
     [by apply auth_auth_valid|].
   iModIntro. iExists (BorrowGS _ _ _ _ γ). iFrame "W". iIntros (??).
-  rewrite borrow_wsat_unseal. iExists ∅. unfold borrow_wsat'. by iFrame.
+  rewrite borrow_wsat_unseal. iExists []. by iFrame.
 Qed.
