nola/util/gmap.v
@@ -3,6 +3,52 @@
 From nola Require Export prelude.
 From stdpp Require Export gmap.
 
+(** ** [list_to_gmap] *)
+
+(** [list_to_gmap]: [list] to [gmap nat] *)
+Fixpoint list_to_gmap' {A : Type} (i : nat) (l : list A) : gmap nat A :=
+  match l with [] => ∅ | x :: l => <[i := x]> (list_to_gmap' (S i) l) end.
+Definition list_to_gmap {A} := list_to_gmap' (A:=A) 0.
+
+(** [!!] over [list_to_gmap] *)
+Lemma lookup_list_to_gmap' {A i l j} :
+  list_to_gmap' (A:=A) i l !! (i + j) = l !! j.
+Proof.
+  move: i j. elim: l; [done|]=>/= y l IH i [|j]/=.
+  { by rewrite Nat.add_0_r lookup_insert. }
+  rewrite lookup_insert_ne; [|lia]. rewrite -(IH (S i)). f_equal. lia.
+Qed.
+Lemma lookup_list_to_gmap {A l i} : list_to_gmap (A:=A) l !! i = l !! i.
+Proof. exact lookup_list_to_gmap'. Qed.
+Lemma lookup_list_to_gmap'_pre {A i l j} :
+  j < i → list_to_gmap' (A:=A) i l !! j = None.
+Proof.
+  move: i j. elim: l; [done|]=>/= a l IH i j ?. apply lookup_insert_None.
+  split; [|lia]. apply IH. lia.
+Qed.
+
+(** [list_to_gmap] over snoc *)
+Lemma list_to_gmap'_snoc {A i l x} :
+  list_to_gmap' (A:=A) i (l ++ [x]) = <[i + length l := x]> (list_to_gmap' i l).
+Proof.
+  move: i. elim: l=>/= [|y l IH] i. { f_equal. lia. }
+  rewrite IH insert_commute; [|lia]. f_equal. lia.
+Qed.
+Lemma list_to_gmap_snoc {A l x} :
+  list_to_gmap (A:=A) (l ++ [x]) = <[length l := x]> (list_to_gmap l).
+Proof. exact list_to_gmap'_snoc. Qed.
+
+(** [list_to_gmap] over [insert] *)
+Lemma list_to_gmap_insert {A l i x} : i < length l →
+  list_to_gmap (A:=A) (<[i := x]> l) = <[i := x]> (list_to_gmap l).
+Proof.
+  move=> ?. apply map_eq=> j. rewrite lookup_list_to_gmap.
+  case (decide (i = j)).
+  - move=> <-. by rewrite lookup_insert list_lookup_insert.
+  - move=> ?. rewrite lookup_insert_ne; [|done].
+    rewrite list_lookup_insert_ne; [|done]. by rewrite lookup_list_to_gmap.
+Qed.
+
 (** ** [map_with], [map_without] and [map_by] *)
 
 (** [map_with m l]: [m] with [l] freshly added *)
